src/program_proof/crash_lockmap_proof.v
@@ -733,7 +733,7 @@ Qed.
 Definition is_lockMap (l: loc) (ghs: list gname) (covered: gset u64) (P Pc: u64 -> iProp Σ) : iProp Σ :=
   ∃ (shards: list loc) (shardslice: Slice.t),
     "#Href" ∷ readonly (l ↦[LockMap :: "shards"] (slice_val shardslice)) ∗
-    "#Hslice" ∷ readonly (is_slice_small shardslice (struct.ptrT lockShard) 1 shards) ∗
+    "#Hslice" ∷ readonly (is_slice_small shardslice ptrT 1 shards) ∗
     "%Hlen" ∷ ⌜ length shards = Z.to_nat NSHARD ⌝ ∗
     "#Hshards" ∷ [∗ list] shardnum ↦ shardloc; shardgh ∈ shards; ghs,
       is_lockShard shardloc shardgh (covered_by_shard shardnum covered) P Pc.
@@ -741,7 +741,7 @@ Definition is_lockMap (l: loc) (ghs: list gname) (covered: gset u64) (P Pc: u64 
 Definition is_free_lockMap (l: loc) : iProp Σ :=
   ∃ (shards: list loc) (shardslice: Slice.t),
     "#Href" ∷ readonly (l ↦[LockMap :: "shards"] (slice_val shardslice)) ∗
-    "#Hslice" ∷ readonly (is_slice_small shardslice (struct.ptrT lockShard) 1 shards) ∗
+    "#Hslice" ∷ readonly (is_slice_small shardslice ptrT 1 shards) ∗
     "%Hlen" ∷ ⌜ length shards = Z.to_nat NSHARD ⌝ ∗
     "Hfree_shards" ∷ [∗ list] shardnum ↦ shardloc ∈ shards, is_free_lockShard shardloc.
 
@@ -776,8 +776,8 @@ Proof.
   wp_pures.
   wp_apply (wp_forUpto (λ (i : u64),
                           ∃ s shardlocs,
-                            "Hvar" ∷ shards ↦[slice.T (refT (struct.t lockShard))] (slice_val s) ∗
-                            "Hslice" ∷ is_slice s (struct.ptrT lockShard) 1 shardlocs ∗
+                            "Hvar" ∷ shards ↦[slice.T ptrT] (slice_val s) ∗
+                            "Hslice" ∷ is_slice s ptrT 1 shardlocs ∗
                             "%Hlen" ∷ ⌜ length shardlocs = int.nat i ⌝ ∗
                             "Hshards" ∷ [∗ list] shardnum ↦ shardloc ∈ shardlocs,
                               is_free_lockShard shardloc)%I
